# (5, 1, 1) F olding from right for list

5.1.1 F olding from right for list . . . . . . . . . . . . . . . . . . . . . . . 163
5.1.1 F olding from right for list
W e defined the fold from right operation for list in chapter 1 as below:
foldrz[] =z
foldrz(x:xs) =x(foldrz xs)
It can be expanded as:
foldrz[x1,x2,...,x n] =x1(x2(...(xnz))...) (5.2)
Many list operations can be realized by folding, for example:
1. Sum:
sum =foldr + 0
2. Theand function, that applies logic and for all Boolean values in a list:
and =foldr^True
This is because:
and [x1,x2,...,x n] =x1^(x2^(...(xn^True ))...)
3. T est if a given element belongs to a list:
elem x xs =foldr (a b7!(a=x)_b)False xs
4. Map:
map f xs =foldr (x ys7!f(x) :ys) []xs
=foldr ((:)f) []xs
5. Filter the elements with a given prediction:
filter f xs =foldr (x ys7!{
f(x) :x:ys
otherwise :ys) []xs164 CHAPTER 5. FUSION
6. Concatenate two lists:
xs+ +ys=foldr (:)ys xs (5.3)
This is because:
[x1,x2,...,x n] + +ys=x1: (x2: (...(xn:ys))...)
7. Concatenate multiple lists:
concat xss =foldr + + []xss
Actually all list operations can be realized by folding (W e proved it in the F-algebra
section in previous chapter), if we can simplify folding, we then can simplify all list
operations.
